Add an injection combinator.
Only in syntax and reduction for now.

theories/AutoSubst/Ast.sig
@@ -25,6 +25,7 @@ tRefl : term -> term -> term
 tIdElim : term -> term -> (bind term , term in term) -> term -> term -> term -> term
 
 tQuote : term -> term -> term
+tInject : term -> term -> term -> term -> term
 tDecide : term -> term -> term -> term
 tReflect : term -> term -> term -> term -> term
 tReify : term -> term -> term -> term -> term
